restructuring so CFA instantiation gets own file

src/Analyze/AbstractInterpCpsK.v
@@ -62,191 +62,6 @@ Section AbstractDomain.
 
 End AbstractDomain.
 
-Module CFA0.
-
-  
-  Section Context_aware.
-    Variable Context : Type.
-    Context {RelDec_c : RelDec (@eq Context)}.
-    Context {AbsTime_c : AbsTime Context RelDec_c}.
-
-    Definition AbstractLocation : Type := var.
-    Inductive PtValue : Type :=
-    | Int : BinNums.Z -> PtValue
-(*    | Ptr : AbstractLocation -> PtValue *)
-    | Tpl : list Value -> PtValue
-    | Clo : Context -> list cont -> list var -> exp -> PtValue
-    with Value := 
-    | Values : list PtValue -> Value (** use set **)
-    | Any    : Value.
-
-    Fixpoint val_leq (v1 v2:Value) : bool :=
-      match v1, v2 with
-        | Any, Any => true
-        | Values vs1, Values vs2 =>
-          List.fold_left (fun acc x => 
-            match find (fun y => ptval_leq x y) vs2 with
-              | None => false
-              | Some _ => acc
-            end) vs1 true
-        | _, Any => true
-        | _, _ => false
-      end
-    with ptval_leq (v1 v2:PtValue) : bool :=
-      match v1, v2 with
-        | Int _, Int _ => true
-        | Tpl vs1, Tpl vs2 => 
-          (fix fold_left2 acc ls1 ls2 :=
-            match ls1, ls2 with
-              | nil, nil => acc
-              | x1::ls1, x2::ls2 =>
-                if val_leq x1 x2 then acc else false
-              | _, _ => false
-            end) true vs1 vs2
-        | Clo c1 ks1 xs1 e1, Clo c2 ks2 xs2 e2 =>
-          rel_dec c1 c2 &&
-          rel_dec ks1 ks2 &&
-          rel_dec xs1 xs2 &&
-          rel_dec e1 e2   
-        | _, _ => false
-      end.
-
-    Definition Domain : Type := alist (var + cont) Value.
-    Definition ProgramPoint : Type := (var + cont)%type.
-
-    Definition bottomValue : Value := Values nil.
-
-    Definition joinValue (v1 v2 : Value) : Value :=
-      match v1 , v2 with
-        | Any , _ => Any
-        | _ , Any => Any
-        | Values x , Values y => Values (x ++ y)
-      end.
-
-    Global Instance AbsDomain_CFA0 : AbsDomain Domain Value Context ProgramPoint :=
-    { lookup  := fun c p d => 
-      match Maps.lookup p d with
-        | None => bottomValue
-        | Some v => v
-      end
-    ; update  := fun c p v d =>
-      match Maps.lookup p d with
-        | None => Maps.add p v d
-        | Some v_old => Maps.add p (joinValue v_old v) d
-      end
-    ; joinA   := joinValue
-    ; bottomA := bottomValue
-    ; topA    := Any
-    ; dom_leq   := fun dom1 dom2 => 
-      fold_alist (fun k v acc => 
-        match Maps.lookup k dom2 with
-          | None => false
-          | Some v' => val_leq v v'
-        end
-        ) true dom1
-    }.
-
-    Global Instance IntValue_Value : IntValue Value :=
-    { injInt := fun v => 
-      match v with 
-        | None => Any
-        | Some v => Values (Int v :: nil)
-      end
-    ; plusA  := fun x y => Any
-    ; minusA := fun x y => Any
-    ; timesA := fun x y => Any
-    ; eqA    := fun _ _ => None
-    ; ltA    := fun _ _ => None
-    }.
-
-    Global Instance BoolValue_Value : BoolValue Value :=
-    { injBool := fun x => Any
-    ; may := fun _ _ => true
-    ; must := fun _ _ => false
-    ; orA := fun _ _ => Any      
-    }.
-
-    Fixpoint list_join_lenAny (ls ls' : list Value) : list Value :=
-      match ls , ls' with
-        | nil , ls' => ls'
-        | ls , nil => ls
-        | l :: ls , l' :: ls' =>
-          joinA l l' :: list_join_lenAny ls ls'
-      end.
-
-    Fixpoint filter_map {A B} (f : A -> option B) (ls : list A) : list B :=
-      match ls with
-        | nil => nil
-        | l :: ls => 
-          match f l with
-            | None => filter_map f ls
-            | Some v => v :: filter_map f ls
-          end
-      end.
-
-    Definition getNats (ls : list PtValue) : list nat :=
-      filter_map (fun x =>
-        match x with
-          | Int BinNums.Z0 => Some 0
-          | Int (BinNums.Zpos n) => Some (BinPos.Pos.to_nat n)
-          | _ => None
-        end) ls.
-
-    Global Instance TplValue_Value : TplValue Value :=
-    { injTuple := fun ls => Values (Tpl ls :: nil)
-    ; projA    := fun n t =>
-      match t with
-        | Any => Any
-        | Values vs =>
-          let ptwise_tuple := List.fold_left (fun acc x => 
-            match x with
-              | Tpl vs => list_join_lenAny vs acc
-              | _ => acc
-            end) vs nil in
-          match n with
-            | Any => List.fold_left joinA ptwise_tuple bottomA 
-            | Values v => 
-              let nats := getNats v in
-              let all := List.map (fun n => 
-                match nth_error ptwise_tuple n with
-                  | None => bottomA
-                  | Some x => x
-                end) nats in
-              List.fold_left joinA all bottomA
-          end
-      end
-    }.
-
-    Definition getClos (ls : list PtValue) : list (Context * list cont * list var * exp) :=
-      filter_map (fun x =>
-        match x with
-          | Clo c xs vs e => Some (c, xs, vs, e)
-          | _ => None
-        end) ls.
-
-    Global Instance FnValue_Value : FnValue Value Context Domain exp :=
-    { injFn := fun c ks xs e => Values (Clo c ks xs e :: nil)
-    ; applyA := fun _ _ aeval dom v ks vs' =>
-      match v with
-        | Any => ret dom (** TODO : think more about this! **)
-        | Values vs =>
-          let clos := getClos vs in
-          foldM (fun x acc => let '(c, ks', xs', e) := x in
-            if eq_dec (List.length ks') (List.length ks) &&
-               eq_dec (List.length xs') (List.length vs) then
-              let ext := List.combine (List.map (fun x => inr x) ks') ks 
-                      ++ List.combine (List.map (fun x => inl x) xs') vs' in
-              let dom' := fold_left (fun acc x => update c (fst x) (snd x) acc) ext dom in 
-              aeval c dom' e
-            else
-              ret acc) (ret dom) clos
-      end
-    }.
-
-  End Context_aware.
-
-End CFA0.
-
 (** NOTE: This is poorly coded
  ** Don't use a random second monad to be cool
  **)
@@ -264,111 +79,109 @@ Section AI.
   Local Open Scope monad_scope.
   Local Open Scope list_scope.
      
-    Section Monadic.
-      Variable m : Type -> Type.
-      Context {Monad_m : Monad m}.
-      Context {Exc_m : MonadExc string m}.
-      Context {Fix_m : MonadFix m}.
-      (** DFS **)
-      Context {State_m : MonadState (alist (C * exp) D) m}.
+  Section Monadic.
+    Variable m : Type -> Type.
+    Context {Monad_m : Monad m}.
+    Context {Exc_m : MonadExc string m}.
+    Context {Fix_m : MonadFix m}.
+    (** DFS **)
+    Context {State_m : MonadState (alist (C * exp) D) m}.
 
-      Definition m' : Type -> Type := 
-        readerT C (stateT D m).
+    Definition m' : Type -> Type := 
+      readerT C (stateT D m).
 
-      Definition runM' {A} (cmd : m' A) (c : C) (d : D) : m (A * D) :=
-        runStateT (runReaderT cmd c) d.
+    Definition runM' {A} (cmd : m' A) (c : C) (d : D) : m (A * D) :=
+      runStateT (runReaderT cmd c) d.
+    
+    Definition eval_op (o : op) : m' V :=
+      match o with
+        | Var_o v =>
+          domain <- get ;;
+          ctx <- ask ;;
+          ret (lookup ctx (inl v) domain)
+        | Con_o c => ret bottomA (** TODO: Not done **)
+        | Int_o i => ret (injInt (Some i))
+        | InitWorld_o => ret bottomA (** TODO: ?? **)
+      end.
+    
+    Section Transfer.
+      Definition illFormed_decl {A} (d : decl) : m A :=
+        raise ("Ill-formed declaration " ++ runShow (show d))%string.
+      
+      Definition eval_decl (d : decl) : m' unit :=
+        v_vA <- 
+        match d return m' (var * V) with
+          | Op_d v o =>
+            oA <- eval_op o ;;
+            ret (v, oA)
+            
+          | Prim_d v p os => 
+            argsA <- mapM eval_op os ;;
+            vA <- match p , argsA return m' V with
+                    | Eq_p , l :: r :: nil =>
+                      ret (injBool (eqA l r))
+                    | Neq_p , l :: r :: nil =>
+                      ret (injBool (map negb (eqA l r)))
+                    | Lt_p , l :: r :: nil =>
+                      ret (injBool (ltA l r))
+                    | Lte_p , l :: r :: nil =>
+                      ret (orA (injBool (ltA l r)) (injBool (eqA l r)))
+                    | Ptr_p , l :: nil => ret (injBool None) (** ?? **)
+                    | Plus_p , l :: r :: nil => ret (plusA l r)
+                    | Minus_p , l :: r :: nil => ret (minusA l r)
+                    | Times_p , l :: r :: nil => ret (timesA l r)
+                    | MkTuple_p , argsA => ret (injTuple argsA)
+                    | Proj_p , l :: r :: nil => ret (projA l r)
+                    | _ , _ => lift (lift (illFormed_decl (Prim_d v p os)))
+                  end ;;
+            ret (v, vA)
 
-      Definition eval_op (o : op) : m' V :=
-        match o with
-          | Var_o v =>
-            domain <- get ;;
+          | Fn_d v ks args body =>
             ctx <- ask ;;
-            ret (lookup ctx (inl v) domain)
-          | Con_o c => ret bottomA (** TODO: Not done **)
-          | Int_o i => ret (injInt (Some i))
-          | InitWorld_o => ret bottomA (** TODO: ?? **)
-        end.
+            ret (v, injFn ctx ks args body)
+            
+          | Bind_d v1 v2 m os =>
+            ret (v1, topA)
+            (*              
+            argsA <- mapM eval_op os ;;
+            admit
+            r <- bindA aeval m argsA ;;
+            match r with
+              | (a1,a2) =>
+                insert v1 a1 ;;
+                insert v2 a2
+            end
+            *)
+        end ;;
+        let '(v, vA) := v_vA in
+        ctx <- ask (T := C) ;;
+        modify (update ctx (inl v) vA) ;;
+        ret tt.
 
-      Section Transfer.
-        Definition illFormed_decl {A} (d : decl) : m A :=
-          raise ("Ill-formed declaration " ++ runShow (show d))%string.
-        
-        Definition eval_decl (d : decl) : m' unit :=
-          v_vA <- 
-          match d return m' (var * V) with
-            | Op_d v o =>
-              oA <- eval_op o ;;
-              ret (v, oA)
-
-            | Prim_d v p os => 
-              argsA <- mapM eval_op os ;;
-              vA <-
-                match p , argsA return m' V with
-                  | Eq_p , l :: r :: nil =>
-                    ret (injBool (eqA l r))
-                  | Neq_p , l :: r :: nil =>
-                    ret (injBool (map negb (eqA l r)))
-                  | Lt_p , l :: r :: nil =>
-                    ret (injBool (ltA l r))
-                  | Lte_p , l :: r :: nil =>
-                    ret (orA (injBool (ltA l r)) (injBool (eqA l r)))
-                  | Ptr_p , l :: nil => ret (injBool None) (** ?? **)
-                  | Plus_p , l :: r :: nil => ret (plusA l r)
-                  | Minus_p , l :: r :: nil => ret (minusA l r)
-                  | Times_p , l :: r :: nil => ret (timesA l r)
-                  | MkTuple_p , argsA => ret (injTuple argsA)
-                  | Proj_p , l :: r :: nil => ret (projA l r)
-                  | _ , _ => lift (lift (illFormed_decl (Prim_d v p os)))
-                end
-              ;;
-              ret (v, vA)
-
-            | Fn_d v ks args body =>
-              ctx <- ask ;;
-              ret (v, injFn ctx ks args body)
-
-            | Bind_d v1 v2 m os =>
-              ret (v1, topA)
-(*              
-              argsA <- mapM eval_op os ;;
-              admit
-              r <- bindA aeval m argsA ;;
-              match r with
-                | (a1,a2) =>
-                  insert v1 a1 ;;
-                  insert v2 a2
+      Definition init_decl (d : decl) : m' unit :=
+        ctx <- ask (T := C) ;;
+        match d return m' _ with
+          | Op_d v _ 
+          | Prim_d v _ _
+          | Fn_d v _ _ _ => 
+            modify (update ctx (inl v) bottomA)
+          | Bind_d v1 v2 _ _ =>
+            modify (update ctx (inl v1) bottomA) ;;
+            modify (update ctx (inl v2) bottomA)
+        end ;;
+        ret tt.
+      
+      Definition aeval : C -> D -> exp -> m D :=
+        mfix3 _ (fun aeval => 
+          fun (ctx : C) (dom : D) (e : exp) =>
+            memo <- gets (Maps.lookup (ctx, e)) ;;
+            let stop :=
+              match memo with
+                | None => false
+                | Some dom' => dom_leq dom dom'
               end
-*)
-          end ;;
-          let '(v, vA) := v_vA in
-          ctx <- ask (T := C) ;;
-          modify (update ctx (inl v) vA) ;;
-          ret tt.
-
-        Definition init_decl (d : decl) : m' unit :=
-          ctx <- ask (T := C) ;;
-          match d return m' _ with
-            | Op_d v _ 
-            | Prim_d v _ _
-            | Fn_d v _ _ _ => 
-              modify (update ctx (inl v) bottomA)
-            | Bind_d v1 v2 _ _ =>
-              modify (update ctx (inl v1) bottomA) ;;
-              modify (update ctx (inl v2) bottomA)
-          end ;;
-          ret tt.
-
-        Definition aeval : C -> D -> exp -> m D :=
-          mfix3 _ (fun aeval => 
-            fun (ctx : C) (dom : D) (e : exp) =>
-              memo <- gets (Maps.lookup (ctx, e)) ;;
-              let stop :=
-                match memo with
-                  | None => false
-                  | Some dom' => dom_leq dom dom'
-                end
-              in
-              if stop then ret dom
+            in
+            if stop then ret dom
               else
                 (fix recur (ctx : C) (dom : D) (e : exp) : m D :=
                   match e return m D with
@@ -462,8 +275,8 @@ Section AI.
                 ret dom
             end).
 *)
+    End Transfer.
+    
+  End Monadic.    
 
-      End Transfer.
-
-    End Monadic.
 End AI.
