src/Analyze/CFA0.v
@@ -1,0 +1,209 @@
+Require Import String List Bool.
+Require Import CoqCompile.CpsK.
+Require Import ExtLib.Structures.Maps.
+Require Import ExtLib.Structures.Monads.
+Require Import ExtLib.Structures.Reducible.
+Require Import ExtLib.Data.Monads.Fuel.
+Require Import ExtLib.Data.Monads.EitherMonad.
+Require Import ExtLib.Data.Monads.ReaderMonad.
+Require Import ExtLib.Data.Monads.StateMonad.
+Require Import ExtLib.Data.Option.
+Require Import ExtLib.Data.Lists.
+Require Import ExtLib.Core.RelDec.
+Require Import ExtLib.Programming.Show.
+Require Import ExtLib.Data.Map.FMapAList.
+Require Import CoqCompile.Analyze.AbstractInterpCpsK.
+
+Import CpsK.CPSK.
+
+Section Context_aware.
+  Variable Context : Type.
+  Context {RelDec_c : RelDec (@eq Context)}.
+  Context {AbsTime_c : AbsTime Context RelDec_c}.
+  
+  Definition AbstractLocation : Type := var.
+  Inductive PtValue : Type :=
+  | Int : BinNums.Z -> PtValue
+  | Tpl : list Value -> PtValue
+  | Clo : Context -> list cont -> list var -> exp -> PtValue
+  with Value := 
+  | Values : list PtValue -> Value (** use set **)
+  | Any    : Value.
+  
+  Fixpoint val_leq (v1 v2:Value) : bool :=
+    match v1, v2 with
+      | Any, Any => true
+      | Values vs1, Values vs2 =>
+        List.fold_left (fun acc x => 
+          match find (fun y => ptval_leq x y) vs2 with
+            | None => false
+            | Some _ => acc
+          end) vs1 true
+      | _, Any => true
+      | _, _ => false
+    end
+  with ptval_leq (v1 v2:PtValue) : bool :=
+    match v1, v2 with
+      | Int _, Int _ => true
+      | Tpl vs1, Tpl vs2 => 
+        (fix fold_left2 acc ls1 ls2 :=
+          match ls1, ls2 with
+            | nil, nil => acc
+            | x1::ls1, x2::ls2 =>
+              if val_leq x1 x2 then acc else false
+            | _, _ => false
+          end) true vs1 vs2
+      | Clo c1 ks1 xs1 e1, Clo c2 ks2 xs2 e2 =>
+        rel_dec c1 c2 &&
+        rel_dec ks1 ks2 &&
+        rel_dec xs1 xs2 &&
+        rel_dec e1 e2   
+      | _, _ => false
+    end.
+  
+  Definition Domain : Type := alist (var + cont) Value.
+  Definition ProgramPoint : Type := (var + cont)%type.
+  
+  Definition bottomValue : Value := Values nil.
+  
+  Definition joinValue (v1 v2 : Value) : Value :=
+    match v1 , v2 with
+      | Any , _ => Any
+      | _ , Any => Any
+      | Values x , Values y => Values (x ++ y)
+    end.
+  
+  Global Instance AbsDomain_CFA0 : AbsDomain Domain Value Context ProgramPoint :=
+  { lookup  := fun c p d => 
+    match Maps.lookup p d with
+      | None => bottomValue
+      | Some v => v
+    end
+  ; update  := fun c p v d =>
+    match Maps.lookup p d with
+      | None => Maps.add p v d
+      | Some v_old => Maps.add p (joinValue v_old v) d
+    end
+  ; joinA   := joinValue
+  ; bottomA := bottomValue
+  ; topA    := Any
+  ; dom_leq   := fun dom1 dom2 => 
+    fold_alist (fun k v acc => 
+      match Maps.lookup k dom2 with
+        | None => false
+        | Some v' => val_leq v v'
+      end
+    ) true dom1
+  }.
+  
+  Global Instance IntValue_Value : IntValue Value :=
+  { injInt := fun v => 
+    match v with 
+      | None => Any
+      | Some v => Values (Int v :: nil)
+    end
+  ; plusA  := fun x y => Any
+  ; minusA := fun x y => Any
+  ; timesA := fun x y => Any
+  ; eqA    := fun _ _ => None
+  ; ltA    := fun _ _ => None
+  }.
+
+  Global Instance BoolValue_Value : BoolValue Value :=
+  { injBool := fun x => Any
+  ; may := fun _ _ => true
+  ; must := fun _ _ => false
+  ; orA := fun _ _ => Any      
+  }.
+
+  Fixpoint list_join_lenAny (ls ls' : list Value) : list Value :=
+    match ls , ls' with
+      | nil , ls' => ls'
+      | ls , nil => ls
+      | l :: ls , l' :: ls' =>
+        joinA l l' :: list_join_lenAny ls ls'
+    end.
+  
+  Fixpoint filter_map {A B} (f : A -> option B) (ls : list A) : list B :=
+    match ls with
+      | nil => nil
+      | l :: ls => 
+        match f l with
+          | None => filter_map f ls
+          | Some v => v :: filter_map f ls
+        end
+    end.
+  
+  Definition getNats (ls : list PtValue) : list nat :=
+    filter_map (fun x =>
+      match x with
+        | Int BinNums.Z0 => Some 0
+        | Int (BinNums.Zpos n) => Some (BinPos.Pos.to_nat n)
+        | _ => None
+      end) ls.
+  
+  Global Instance TplValue_Value : TplValue Value :=
+  { injTuple := fun ls => Values (Tpl ls :: nil)
+  ; projA    := fun n t =>
+    match t with
+      | Any => Any
+      | Values vs =>
+        let ptwise_tuple := List.fold_left (fun acc x => 
+          match x with
+            | Tpl vs => list_join_lenAny vs acc
+            | _ => acc
+          end) vs nil in
+        match n with
+          | Any => List.fold_left joinA ptwise_tuple bottomA 
+          | Values v => 
+            let nats := getNats v in
+            let all := List.map (fun n => 
+              match nth_error ptwise_tuple n with
+                | None => bottomA
+                | Some x => x
+              end) nats in
+            List.fold_left joinA all bottomA
+        end
+    end
+  }.
+
+  Definition getClos (ls : list PtValue) : list (Context * list cont * list var * exp) :=
+    filter_map (fun x =>
+      match x with
+        | Clo c xs vs e => Some (c, xs, vs, e)
+        | _ => None
+      end) ls.
+  
+  Global Instance FnValue_Value : FnValue Value Context Domain exp :=
+  { injFn := fun c ks xs e => Values (Clo c ks xs e :: nil)
+  ; applyA := fun _ _ aeval dom v ks vs' =>
+    match v with
+      | Any => ret dom (** TODO : think more about this! **)
+      | Values vs =>
+        let clos := getClos vs in
+          foldM (fun x acc => let '(c, ks', xs', e) := x in
+          if eq_dec (List.length ks') (List.length ks) &&
+             eq_dec (List.length xs') (List.length vs) then
+            let ext := List.combine (List.map (fun x => inr x) ks') ks 
+                    ++ List.combine (List.map (fun x => inl x) xs') vs' in
+            let dom' := fold_left (fun acc x => update c (fst x) (snd x) acc) ext dom in 
+              aeval c dom' e
+            else
+              ret acc) (ret dom) clos
+    end
+  }.
+  
+  Set Printing All.
+  Print aeval.
+
+  Local Open Scope monad_scope.
+
+  Print eitherT.
+
+  Definition cfa_0 : Domain.
+  refine (
+    let m := eitherT string (stateT (alist (Context*exp) Domain) (fuel (sum string))) in
+    let blah := aeval Domain Context _ in _
+  ).
+
+End Context_aware.
